fix captured generic direct proof recovery

fixtures/TypeChecker.ml
@@ -15547,6 +15547,73 @@ let check_expr_root_shadow_store_safe_narrow_summary_checked env _UU03a9_ n r _U
     (of_num_uint (UIntDecimal (D1 (D0 (D0 (D0 (D0 Nil))))))) env _UU03a9_ n r
     (sctx_of_ctx _UU0393_) e
 
+(** val check_fn_root_shadow_generic_direct_store_safe_summary_target :
+    global_env -> fn_def -> ident -> ty list -> expr list -> expr -> bool **)
+
+let check_fn_root_shadow_generic_direct_store_safe_summary_target env fdef fname type_args args synthetic_body =
+  (&&) (store_safe_function_value_call_args_b env args)
+    (match lookup_fn_b fname env.env_fns with
+     | Some callee ->
+       (&&) (Nat.eqb (length type_args) callee.fn_type_params)
+         (match check_struct_bounds
+                  (global_env_with_local_bounds env fdef.fn_bounds)
+                  callee.fn_bounds type_args with
+          | Some _ -> false
+          | None ->
+            let callee_body_env =
+              global_env_with_local_bounds env
+                (subst_type_params_trait_bounds type_args callee.fn_bounds)
+            in
+            (match infer_core_env_roots_shadow_safe callee_body_env
+                     callee.fn_outlives callee.fn_lifetimes
+                     (initial_root_env_for_fn callee)
+                     (subst_type_params_ctx type_args (fn_body_ctx callee))
+                     (subst_type_params_expr type_args callee.fn_body) with
+             | Infer_ok p ->
+               let (p0, roots_callee) = p in
+               let (p1, r_callee) = p0 in
+               let (t_callee, _) = p1 in
+               (match infer_env_roots_shadow_safe env callee
+                        (initial_root_env_for_fn callee) with
+                | Infer_ok _ ->
+                  (match infer_env_roots_shadow_safe env
+                           (fn_with_body fdef synthetic_body)
+                           (initial_root_env_for_fn fdef) with
+                   | Infer_ok p3 ->
+                     let (p4, roots) = p3 in
+                     let (p5, r_out) = p4 in
+                     let (t_body, _) = p5 in
+                     (&&)
+                       ((&&)
+                         ((&&)
+                           ((&&)
+                             ((&&)
+                               ((&&)
+                                 ((&&)
+                                   (preservation_ready_expr_b
+                                     (subst_type_params_expr type_args
+                                       callee.fn_body))
+                                   (check_callee_body_root_shadow_store_safe_narrow_summary_instantiated
+                                     env callee type_args))
+                                 (ty_compatible_b callee.fn_outlives t_callee
+                                   (subst_type_params_ty type_args
+                                     callee.fn_ret)))
+                               (fn_params_roots_exclude_b
+                                 (apply_type_params type_args
+                                   callee.fn_params)
+                                 roots_callee))
+                             (fn_params_root_env_excludes_b
+                               (apply_type_params type_args callee.fn_params)
+                               r_callee))
+                           (ty_compatible_b fdef.fn_outlives t_body
+                             fdef.fn_ret))
+                         (fn_params_roots_exclude_b fdef.fn_params roots))
+                       (fn_params_root_env_excludes_b fdef.fn_params r_out)
+                   | Infer_err _ -> false)
+                | Infer_err _ -> false)
+             | Infer_err _ -> false))
+     | None -> false)
+
 (** val check_fn_root_shadow_generic_direct_store_safe_summary :
     global_env -> fn_def -> bool **)
 
@@ -15556,70 +15623,8 @@ let check_fn_root_shadow_generic_direct_store_safe_summary env fdef =
     let (p0, synthetic_body) = p in
     let (p1, args) = p0 in
     let (fname, type_args) = p1 in
-    (&&) (store_safe_function_value_call_args_b env args)
-      (match lookup_fn_b fname env.env_fns with
-       | Some callee ->
-         (&&) (Nat.eqb (length type_args) callee.fn_type_params)
-           (match check_struct_bounds
-                    (global_env_with_local_bounds env fdef.fn_bounds)
-                    callee.fn_bounds type_args with
-            | Some _ -> false
-            | None ->
-              let callee_body_env =
-                global_env_with_local_bounds env
-                  (subst_type_params_trait_bounds type_args callee.fn_bounds)
-              in
-              (match infer_core_env_roots_shadow_safe callee_body_env
-                       callee.fn_outlives callee.fn_lifetimes
-                       (initial_root_env_for_fn callee)
-                       (subst_type_params_ctx type_args (fn_body_ctx callee))
-                       (subst_type_params_expr type_args callee.fn_body) with
-               | Infer_ok p2 ->
-                 let (p3, roots_callee) = p2 in
-                 let (p4, r_callee) = p3 in
-                 let (t_callee, _) = p4 in
-                 (match infer_env_roots_shadow_safe env callee
-                          (initial_root_env_for_fn callee) with
-                  | Infer_ok _ ->
-                    (match infer_env_roots_shadow_safe env
-                             (fn_with_body fdef synthetic_body)
-                             (initial_root_env_for_fn fdef) with
-                     | Infer_ok p5 ->
-                       let (p6, roots) = p5 in
-                       let (p7, r_out) = p6 in
-                       let (t_body, _) = p7 in
-                       (&&)
-                         ((&&)
-                           ((&&)
-                             ((&&)
-                               ((&&)
-                                 ((&&)
-                                   ((&&)
-                                     (preservation_ready_expr_b
-                                       (subst_type_params_expr type_args
-                                         callee.fn_body))
-                                     (check_callee_body_root_shadow_store_safe_narrow_summary_instantiated
-                                       env callee type_args))
-                                   (ty_compatible_b callee.fn_outlives
-                                     t_callee
-                                     (subst_type_params_ty type_args
-                                       callee.fn_ret)))
-                                 (fn_params_roots_exclude_b
-                                   (apply_type_params type_args
-                                     callee.fn_params)
-                                   roots_callee))
-                               (fn_params_root_env_excludes_b
-                                 (apply_type_params type_args
-                                   callee.fn_params)
-                                 r_callee))
-                             (ty_compatible_b fdef.fn_outlives t_body
-                               fdef.fn_ret))
-                           (fn_params_roots_exclude_b fdef.fn_params roots))
-                         (fn_params_root_env_excludes_b fdef.fn_params r_out)
-                     | Infer_err _ -> false)
-                  | Infer_err _ -> false)
-               | Infer_err _ -> false))
-       | None -> false)
+    check_fn_root_shadow_generic_direct_store_safe_summary_target env fdef
+      fname type_args args synthetic_body
   | None -> false
 
 (** val check_fn_root_shadow_no_capture_direct_call_component_store_safe_summary :
